vale/code/arch/x64/X64.Vale.Decls.fsti
@@ -36,63 +36,6 @@ let va_reveal_opaque (s:string) = norm_spec [zeta; delta_only [s]]
 let va_if (#a:Type) (b:bool) (x:(_:unit{b}) -> GTot a) (y:(_:unit{~b}) -> GTot a) : GTot a =
   if b then x () else y ()
 
-(* Define a tainted operand to wrap the base operand type *)
-[@va_qattr]
-type tainted_operand:eqtype =
-| TConst: n:int -> tainted_operand
-| TReg: r:reg -> tainted_operand
-| TMem: m:maddr -> t:taint -> tainted_operand
-| TStack: m:maddr -> t:taint -> tainted_operand
-
-
-[@va_qattr]
-type tainted_operand128:eqtype =
-| TReg128: x:xmm -> tainted_operand128
-| TMem128: m:maddr -> t:taint -> tainted_operand128
-
-[@va_qattr]
-unfold let t_op_to_op (t:tainted_operand) : operand =
-  match t with
-  | TConst n -> OConst n
-  | TReg r -> OReg r
-  | TMem m _ -> OMem m
-  | TStack m _ -> OStack m
-  
-
-[@va_qattr]
-unfold let t_op_to_op128 (t:tainted_operand128) : mov128_op =
-  match t with
-  | TReg128 r -> Mov128Xmm r
-  | TMem128 m _ -> Mov128Mem m
-
-let get_taint (t:tainted_operand) : taint =
-  match t with
-  | TConst _ -> Public
-  | TReg _ -> Public
-  | TMem _ t -> t
-  | TStack _ t -> t
-
-let get_taint128 (t:tainted_operand128) : taint =
-  match t with
-  | TReg128 _ -> Public
-  | TMem128 _ t -> t
-
-let extract_taint (o1 o2:tainted_operand) : taint =
-  if TMem? o1 || TStack? o1 then get_taint o1
-  else if TMem? o2 || TStack? o2 then get_taint o2
-  else Public
-
-let extract_taint128 (o1 o2:tainted_operand128) : taint =
-  if TMem128? o1 then TMem128?.t o1
-  else if TMem128? o2 then TMem128?.t o2
-  else Public
-
-let extract_taint3 (o1 o2 o3:tainted_operand) : taint =
-  if TMem? o1 || TStack? o1 then get_taint o1
-  else if TMem? o2 || TStack? o2 then get_taint o2
-  else if TMem? o3 || TStack? o3 then get_taint o3
-  else Public
-
 (* Type aliases *)
 unfold let va_bool = bool
 unfold let va_prop = prop0
@@ -107,24 +50,24 @@ unfold let va_codes = list va_code
 let va_tl (cs:va_codes) : Ghost va_codes (requires Cons? cs) (ensures fun tl -> tl == Cons?.tl cs) = Cons?.tl cs
 unfold let va_state = state
 val va_fuel : Type0
-unfold let va_operand = tainted_operand
+unfold let va_operand = operand
 unfold let va_operand_opr64 = va_operand
-let va_reg_operand = o:va_operand{OReg? (t_op_to_op o)}
-let va_operand_reg_opr64 = o:va_operand{OReg? (t_op_to_op o)}
+let va_reg_operand = o:va_operand{OReg? o}
+let va_operand_reg_opr64 = o:va_operand{OReg? o}
 unfold let va_dst_operand = o:va_operand
 unfold let va_operand_dst_opr64 = o:va_operand
 unfold let va_shift_amt = o:va_operand
 unfold let va_operand_shift_amt64 = o:va_operand
-unfold let va_cmp = o:va_operand{not (TMem? o)}
+unfold let va_cmp = o:va_operand{not (OMem? o)}
 unfold let va_register = reg
 unfold let va_operand_xmm = xmm
-unfold let va_operand128 = tainted_operand128
+unfold let va_operand128 = operand128
 unfold let va_operand_opr128 = va_operand128
 
 [@va_qattr] unfold let va_expand_state (s:state) : state = state_eta s
 
 (* Abbreviations *)
-unfold let get_reg (o:va_reg_operand) : reg = OReg?.r (t_op_to_op o)
+unfold let get_reg (o:va_reg_operand) : reg = OReg?.r o
 unfold let buffer_readable (#t:M.base_typ) (h:M.mem) (b:M.buffer t) : GTot prop0 = M.buffer_readable #t h b
 unfold let buffer_writeable (#t:M.base_typ) (b:M.buffer t) : GTot prop0 = M.buffer_writeable #t b
 unfold let buffer_length (#t:M.base_typ) (b:M.buffer t) = M.buffer_length #t b
@@ -169,64 +112,70 @@ let valid_mem_operand128 (addr:int) (t:taint) (s_mem:M.mem) (s_memTaint:M.memtai
     valid_maddr128 addr s_mem s_memTaint b index t
 
 [@va_qattr]
-let valid_operand (t:tainted_operand) (s:state) : prop0 =
-  X64.Vale.State.valid_src_operand (t_op_to_op t) s /\
-  (match t with TMem m t -> valid_mem_operand (eval_maddr m s) t s.mem s.memTaint
-         | TStack m t -> S.valid_taint_stack64 (eval_maddr m s) t s.stackTaint
-         | _ -> True)
+let valid_operand (o:operand) (s:state) : prop0 =
+  X64.Vale.State.valid_src_operand o s /\
+  ( match o with
+    | OMem (m, t) -> valid_mem_operand (eval_maddr m s) t s.mem s.memTaint
+    | OStack (m, t) -> S.valid_taint_stack64 (eval_maddr m s) t s.stackTaint
+    | _ -> True
+  )
 
 [@va_qattr]
-let valid_operand128 (t:tainted_operand128) (s:state) : prop0 =
-  X64.Vale.State.valid_src_operand128 (t_op_to_op128 t) s /\
-  (match t with TMem128 m t -> valid_mem_operand128 (eval_maddr m s) t s.mem s.memTaint | _ -> True)
+let valid_operand128 (o:operand128) (s:state) : prop0 =
+  X64.Vale.State.valid_src_operand128 o s /\
+  ( match o with
+    | OMem128 (m, t) -> valid_mem_operand128 (eval_maddr m s) t s.mem s.memTaint
+    | OStack128 (m, t) -> S.valid_taint_stack128 (eval_maddr m s) t s.stackTaint
+    | _ -> True
+  )
 
 (* Constructors *)
 val va_fuel_default : unit -> va_fuel
-[@va_qattr] unfold let va_op_operand_reg (r:reg) : va_operand = TReg r
+[@va_qattr] unfold let va_op_operand_reg (r:reg) : va_operand = OReg r
 [@va_qattr] unfold let va_op_xmm_xmm (x:xmm) : va_operand_xmm = x
-[@va_qattr] unfold let va_op_opr_reg (r:reg) : va_operand = TReg r
-[@va_qattr] unfold let va_op_opr64_reg (r:reg) : va_operand = TReg r
-[@va_qattr] unfold let va_op_reg64_reg (r:reg) : va_operand = TReg r
-[@va_qattr] unfold let va_op_opr128_xmm (x:xmm) : va_operand128 = TReg128 x
-[@va_qattr] unfold let va_const_operand (n:int) = TConst n
-[@va_qattr] unfold let va_const_opr64 (n:int) = TConst n
-[@va_qattr] unfold let va_const_shift_amt (n:int) : va_shift_amt = TConst n
-[@va_qattr] unfold let va_const_shift_amt64 (n:int) : va_shift_amt = TConst n
-[@va_qattr] unfold let va_op_shift_amt_reg (r:reg) : va_shift_amt = TReg r
-[@va_qattr] unfold let va_op_shift_amt64_reg (r:reg) : va_shift_amt = TReg r
-[@va_qattr] unfold let va_op_cmp_reg (r:reg) : va_cmp = TReg r
-[@va_qattr] unfold let va_const_cmp (n:int) : va_cmp = TConst n
+[@va_qattr] unfold let va_op_opr_reg (r:reg) : va_operand = OReg r
+[@va_qattr] unfold let va_op_opr64_reg (r:reg) : va_operand = OReg r
+[@va_qattr] unfold let va_op_reg64_reg (r:reg) : va_operand = OReg r
+[@va_qattr] unfold let va_op_opr128_xmm (x:xmm) : va_operand128 = OReg128 x
+[@va_qattr] unfold let va_const_operand (n:int) = OConst n
+[@va_qattr] unfold let va_const_opr64 (n:int) = OConst n
+[@va_qattr] unfold let va_const_shift_amt (n:int) : va_shift_amt = OConst n
+[@va_qattr] unfold let va_const_shift_amt64 (n:int) : va_shift_amt = OConst n
+[@va_qattr] unfold let va_op_shift_amt_reg (r:reg) : va_shift_amt = OReg r
+[@va_qattr] unfold let va_op_shift_amt64_reg (r:reg) : va_shift_amt = OReg r
+[@va_qattr] unfold let va_op_cmp_reg (r:reg) : va_cmp = OReg r
+[@va_qattr] unfold let va_const_cmp (n:int) : va_cmp = OConst n
 [@va_qattr] unfold let va_coerce_reg_opr64_to_cmp (r:va_operand_reg_opr64) : va_cmp = r
-[@va_qattr] unfold let va_coerce_register_to_operand (r:va_register) : va_operand = TReg r
-[@va_qattr] unfold let va_coerce_operand_to_reg_operand (o:va_operand{OReg? (t_op_to_op o)}) : va_reg_operand = o
-[@va_qattr] unfold let va_coerce_dst_operand_to_reg_operand (o:va_dst_operand{OReg? (t_op_to_op o)}) : va_reg_operand = o
+[@va_qattr] unfold let va_coerce_register_to_operand (r:va_register) : va_operand = OReg r
+[@va_qattr] unfold let va_coerce_operand_to_reg_operand (o:va_operand{OReg? o}) : va_reg_operand = o
+[@va_qattr] unfold let va_coerce_dst_operand_to_reg_operand (o:va_dst_operand{OReg? o}) : va_reg_operand = o
 [@va_qattr] unfold let va_coerce_reg_opr64_to_dst_opr64 (o:va_operand_reg_opr64) : va_operand_dst_opr64 = o
 [@va_qattr] unfold let va_coerce_reg_opr64_to_opr64 (o:va_operand_reg_opr64) : va_operand_opr64 = o
-[@va_qattr] unfold let va_coerce_operand_to_cmp (o:va_operand{not (TMem? o)}) : va_cmp = o
-[@va_qattr] unfold let va_coerce_opr64_to_cmp (o:va_operand{not (TMem? o)}) : va_cmp = o
+[@va_qattr] unfold let va_coerce_operand_to_cmp (o:va_operand{not (OMem? o)}) : va_cmp = o
+[@va_qattr] unfold let va_coerce_opr64_to_cmp (o:va_operand{not (OMem? o)}) : va_cmp = o
 [@va_qattr] unfold let va_op_register (r:reg) : va_register = r
-[@va_qattr] unfold let va_op_reg_oprerand_reg (r:reg) : va_reg_operand = TReg r
-[@va_qattr] unfold let va_op_reg_opr64_reg (r:reg) : va_reg_operand = TReg r
-[@va_qattr] unfold let va_op_dst_operand_reg (r:reg) : va_dst_operand = TReg r
-[@va_qattr] unfold let va_op_dst_opr64_reg (r:reg) : va_dst_operand = TReg r
+[@va_qattr] unfold let va_op_reg_oprerand_reg (r:reg) : va_reg_operand = OReg r
+[@va_qattr] unfold let va_op_reg_opr64_reg (r:reg) : va_reg_operand = OReg r
+[@va_qattr] unfold let va_op_dst_operand_reg (r:reg) : va_dst_operand = OReg r
+[@va_qattr] unfold let va_op_dst_opr64_reg (r:reg) : va_dst_operand = OReg r
 [@va_qattr] unfold let va_coerce_operand_to_dst_operand (o:va_operand) : va_dst_operand = o
 [@va_qattr] unfold let va_coerce_dst_operand_to_operand (o:va_dst_operand) : va_operand = o
 [@va_qattr] unfold let va_coerce_dst_opr64_to_opr64 (o:va_dst_operand) : va_operand = o
-[@va_qattr] unfold let va_coerce_xmm_to_opr128 (x:xmm) : va_operand128 = TReg128 x
+[@va_qattr] unfold let va_coerce_xmm_to_opr128 (x:xmm) : va_operand128 = OReg128 x
 
 [@va_qattr]
 unfold let va_opr_code_Mem (o:va_operand) (offset:int) (t:taint) : va_operand =
   match o with
-  | TConst n -> TMem (MConst (n + offset)) t
-  | TReg r -> TMem (MReg r offset) t
-  | _ -> TMem (MConst 42) t
+  | OConst n -> OMem (MConst (n + offset), t)
+  | OReg r -> OMem (MReg r offset, t)
+  | _ -> OMem (MConst 42, t)
 
 val va_opr_lemma_Mem (s:va_state) (base:va_operand) (offset:int) (b:M.buffer64) (index:int) (t:taint) : Lemma
   (requires
-    TReg? base /\
+    OReg? base /\
     valid_src_addr s.mem b index /\
     M.valid_taint_buf64 b s.mem s.memTaint t /\
-    eval_operand (t_op_to_op base) s + offset == M.buffer_addr b s.mem + 8 `op_Multiply` index
+    eval_operand base s + offset == M.buffer_addr b s.mem + 8 `op_Multiply` index
   )
   (ensures
     valid_operand (va_opr_code_Mem base offset t) s /\
@@ -236,29 +185,29 @@ val va_opr_lemma_Mem (s:va_state) (base:va_operand) (offset:int) (b:M.buffer64) 
 [@va_qattr]
 unfold let va_opr_code_Stack (o:va_operand) (offset:int) (t:taint) : va_operand =
   match o with
-  | TConst n -> TStack (MConst (n + offset)) t
-  | TReg r -> TStack (MReg r offset) t
-  | _ -> TStack (MConst 42) t
+  | OConst n -> OStack (MConst (n + offset), t)
+  | OReg r -> OStack (MReg r offset, t)
+  | _ -> OStack (MConst 42, t)
 
 val va_opr_lemma_Stack (s:va_state) (base:va_operand) (offset:int) (t:taint) : Lemma
   (requires
-    TReg? base /\
-    S.valid_stack_slot64 (eval_operand (t_op_to_op base) s + offset) s.stack t s.stackTaint
+    OReg? base /\
+    S.valid_stack_slot64 (eval_operand base s + offset) s.stack t s.stackTaint
   )
   (ensures True)
 
 [@va_qattr]
 unfold let va_opr_code_Mem128 (o:va_operand) (offset:int) (t:taint) : va_operand128 =
   match o with
-  | TReg r -> TMem128 (MReg r offset) t
-  | _ -> TMem128 (MConst 42) t
+  | OReg r -> OMem128 (MReg r offset, t)
+  | _ -> OMem128 (MConst 42, t)
 
 val va_opr_lemma_Mem128 (s:va_state) (base:va_operand) (offset:int) (t:taint) (b:M.buffer128) (index:int) : Lemma
   (requires
-    TReg? base /\
+    OReg? base /\
     valid_src_addr s.mem b index /\
     M.valid_taint_buf128 b s.mem s.memTaint t /\
-    eval_operand (t_op_to_op base) s + offset == M.buffer_addr b s.mem + 16 `op_Multiply` index
+    eval_operand base s + offset == M.buffer_addr b s.mem + 16 `op_Multiply` index
   )
   (ensures
     valid_operand128 (va_opr_code_Mem128 base offset t) s /\
@@ -268,24 +217,24 @@ val va_opr_lemma_Mem128 (s:va_state) (base:va_operand) (offset:int) (t:taint) (b
 val taint_at (memTaint:M.memtaint) (addr:int) : taint
 
 (* Evaluation *)
-[@va_qattr] unfold let va_eval_opr64        (s:va_state) (o:va_operand)     : GTot nat64 = eval_operand (t_op_to_op o) s
-[@va_qattr] unfold let va_eval_dst_opr64    (s:va_state) (o:va_dst_operand) : GTot nat64 = eval_operand (t_op_to_op o) s
-[@va_qattr] unfold let va_eval_shift_amt64  (s:va_state) (o:va_shift_amt)   : GTot nat64 = eval_operand (t_op_to_op o) s
-[@va_qattr] unfold let va_eval_cmp_uint64   (s:va_state) (r:va_cmp)         : GTot nat64 = eval_operand (t_op_to_op r) s
+[@va_qattr] unfold let va_eval_opr64        (s:va_state) (o:va_operand)     : GTot nat64 = eval_operand o s
+[@va_qattr] unfold let va_eval_dst_opr64    (s:va_state) (o:va_dst_operand) : GTot nat64 = eval_operand o s
+[@va_qattr] unfold let va_eval_shift_amt64  (s:va_state) (o:va_shift_amt)   : GTot nat64 = eval_operand o s
+[@va_qattr] unfold let va_eval_cmp_uint64   (s:va_state) (r:va_cmp)         : GTot nat64 = eval_operand r s
 [@va_qattr] unfold let va_eval_reg64        (s:va_state) (r:va_register)    : GTot nat64 = eval_reg r s
-[@va_qattr] unfold let va_eval_reg_opr64    (s:va_state) (o:va_operand)     : GTot nat64 = eval_operand (t_op_to_op o) s
+[@va_qattr] unfold let va_eval_reg_opr64    (s:va_state) (o:va_operand)     : GTot nat64 = eval_operand o s
 [@va_qattr] unfold let va_eval_xmm          (s:va_state) (x:xmm)            : GTot quad32 = eval_xmm x s
-[@va_qattr] unfold let va_eval_opr128       (s:va_state) (o:va_operand128)  : GTot quad32 = eval_operand128 (t_op_to_op128 o) s
+[@va_qattr] unfold let va_eval_opr128       (s:va_state) (o:va_operand128)  : GTot quad32 = eval_operand128 o s
 
 (* Predicates *)
 [@va_qattr] unfold let va_is_src_opr64 (o:va_operand) (s:va_state) = valid_operand o s
-[@va_qattr] let va_is_dst_opr64 (o:va_operand) (s:va_state) = match (t_op_to_op o) with OReg r -> not (r = rRsp ) | _ -> false
+[@va_qattr] let va_is_dst_opr64 (o:va_operand) (s:va_state) = match o with OReg r -> not (r = rRsp ) | _ -> false
 [@va_qattr] unfold let va_is_dst_dst_opr64 (o:va_dst_operand) (s:va_state) = va_is_dst_opr64 o s
 [@va_qattr] unfold let va_is_src_reg (r:reg) (s:va_state) = True
 [@va_qattr] unfold let va_is_dst_reg (r:reg) (s:va_state) = True
 [@va_qattr] unfold let va_is_src_shift_amt64 (o:va_operand) (s:va_state) = valid_operand o s /\ (va_eval_shift_amt64 s o) < 64
-[@va_qattr] unfold let va_is_src_reg_opr64 (o:va_operand) (s:va_state) = OReg? (t_op_to_op o)
-[@va_qattr] unfold let va_is_dst_reg_opr64 (o:va_operand) (s:va_state) = OReg? (t_op_to_op o) /\ not (rRsp = (OReg?.r (t_op_to_op o)))
+[@va_qattr] unfold let va_is_src_reg_opr64 (o:va_operand) (s:va_state) = OReg? o
+[@va_qattr] unfold let va_is_dst_reg_opr64 (o:va_operand) (s:va_state) = OReg? o /\ not (rRsp = (OReg?.r o))
 [@va_qattr] unfold let va_is_src_xmm (x:xmm) (s:va_state) = True
 [@va_qattr] unfold let va_is_dst_xmm (x:xmm) (s:va_state) = True
 [@va_qattr] unfold let va_is_src_opr128 (o:va_operand128) (s:va_state) = valid_operand128 o s
@@ -325,11 +274,11 @@ val taint_at (memTaint:M.memtaint) (addr:int) : taint
 
 [@va_qattr]
 let va_update_operand (o:va_operand) (sM:va_state) (sK:va_state) : va_state =
-  match (t_op_to_op o) with
+  match o with
   | OConst n -> sK
   | OReg r -> va_update_reg r sM sK
-  | OMem m -> va_update_mem sM sK
-  | OStack m -> va_update_stack sM sK
+  | OMem (m, _) -> va_update_mem sM sK
+  | OStack (m, _) -> va_update_stack sM sK
 
 [@va_qattr] unfold
 let va_update_dst_operand (o:va_operand) (sM:va_state) (sK:va_state) : va_state =
@@ -366,24 +315,24 @@ let va_upd_operand_xmm (x:xmm) (v:quad32) (s:state) : state =
 
 [@va_qattr]
 let va_upd_operand_dst_opr64 (o:va_operand) (v:nat64) (s:state) =
-  match (t_op_to_op o) with
+  match o with
   | OConst n -> s
   | OReg r -> update_reg r v s
-  | OMem m -> s // TODO: support destination memory operands
-  | OStack m -> s // TODO: support destination stack operands
+  | OMem (m, _) -> s // TODO: support destination memory operands
+  | OStack (m, _) -> s // TODO: support destination stack operands
 
 [@va_qattr]
 let va_upd_operand_reg_opr64 (o:va_operand) (v:nat64) (s:state) =
-  match (t_op_to_op o) with
+  match o with
   | OConst n -> s
   | OReg r -> update_reg r v s
-  | OMem m -> s
-  | OStack m -> s
+  | OMem (m, _) -> s
+  | OStack (m, _) -> s
 
 let va_lemma_upd_update (sM:state) : Lemma
   (
-    (forall (sK:state) (o:va_operand).{:pattern (va_update_operand_dst_opr64 o sM sK)} va_is_dst_dst_opr64 o sK ==> va_update_operand_dst_opr64 o sM sK == va_upd_operand_dst_opr64 o (eval_operand (t_op_to_op o) sM) sK) /\
-    (forall (sK:state) (o:va_operand).{:pattern (va_update_operand_reg_opr64 o sM sK)} va_is_dst_reg_opr64 o sK ==> va_update_operand_reg_opr64 o sM sK == va_upd_operand_reg_opr64 o (eval_operand (t_op_to_op o) sM) sK) /\
+    (forall (sK:state) (o:va_operand).{:pattern (va_update_operand_dst_opr64 o sM sK)} va_is_dst_dst_opr64 o sK ==> va_update_operand_dst_opr64 o sM sK == va_upd_operand_dst_opr64 o (eval_operand o sM) sK) /\
+    (forall (sK:state) (o:va_operand).{:pattern (va_update_operand_reg_opr64 o sM sK)} va_is_dst_reg_opr64 o sK ==> va_update_operand_reg_opr64 o sM sK == va_upd_operand_reg_opr64 o (eval_operand o sM) sK) /\
     (forall (sK:state) (x:xmm).{:pattern (va_update_operand_xmm x sM sK)} va_update_operand_xmm x sM sK == va_upd_operand_xmm x (eval_xmm x sM) sK)
   )
   = ()
@@ -397,12 +346,12 @@ unfold let va_Block (block:va_codes) : va_code = Block block
 unfold let va_IfElse (ifCond:ocmp) (ifTrue:va_code) (ifFalse:va_code) : va_code = IfElse ifCond ifTrue ifFalse
 unfold let va_While (whileCond:ocmp) (whileBody:va_code) : va_code = While whileCond whileBody
 
-val va_cmp_eq (o1:va_operand{ not (TMem? o1 || TStack? o1) }) (o2:va_operand{ not (TMem? o2 || TStack? o2) }) : ocmp
-val va_cmp_ne (o1:va_operand{ not (TMem? o1 || TStack? o1) }) (o2:va_operand{ not (TMem? o2 || TStack? o2) }) : ocmp
-val va_cmp_le (o1:va_operand{ not (TMem? o1 || TStack? o1) }) (o2:va_operand{ not (TMem? o2 || TStack? o2) }) : ocmp
-val va_cmp_ge (o1:va_operand{ not (TMem? o1 || TStack? o1) }) (o2:va_operand{ not (TMem? o2 || TStack? o2) }) : ocmp
-val va_cmp_lt (o1:va_operand{ not (TMem? o1 || TStack? o1) }) (o2:va_operand{ not (TMem? o2 || TStack? o2) }) : ocmp
-val va_cmp_gt (o1:va_operand{ not (TMem? o1 || TStack? o1) }) (o2:va_operand{ not (TMem? o2 || TStack? o2) }) : ocmp
+val va_cmp_eq (o1:va_operand{ not (OMem? o1 || OStack? o1) }) (o2:va_operand{ not (OMem? o2 || OStack? o2) }) : ocmp
+val va_cmp_ne (o1:va_operand{ not (OMem? o1 || OStack? o1) }) (o2:va_operand{ not (OMem? o2 || OStack? o2) }) : ocmp
+val va_cmp_le (o1:va_operand{ not (OMem? o1 || OStack? o1) }) (o2:va_operand{ not (OMem? o2 || OStack? o2) }) : ocmp
+val va_cmp_ge (o1:va_operand{ not (OMem? o1 || OStack? o1) }) (o2:va_operand{ not (OMem? o2 || OStack? o2) }) : ocmp
+val va_cmp_lt (o1:va_operand{ not (OMem? o1 || OStack? o1) }) (o2:va_operand{ not (OMem? o2 || OStack? o2) }) : ocmp
+val va_cmp_gt (o1:va_operand{ not (OMem? o1 || OStack? o1) }) (o2:va_operand{ not (OMem? o2 || OStack? o2) }) : ocmp
 
 unfold let va_get_block (c:va_code{Block? c}) : va_codes = Block?.block c
 unfold let va_get_ifCond (c:va_code{IfElse? c}) : ocmp = IfElse?.ifCond c
@@ -554,62 +503,62 @@ unfold let va_evalCond (b:ocmp) (s:va_state) : GTot bool = eval_ocmp s b
 
 val valid_ocmp : c:ocmp -> s:va_state -> GTot bool
 
-val lemma_cmp_eq : s:va_state -> o1:va_operand{ not (TMem? o1 || TStack? o1) } -> o2:va_operand{ not (TMem? o2 || TStack? o2) } -> Lemma
+val lemma_cmp_eq : s:va_state -> o1:va_operand{ not (OMem? o1 || OStack? o1) } -> o2:va_operand{ not (OMem? o2 || OStack? o2) } -> Lemma
   (requires True)
   (ensures  (eval_ocmp s (va_cmp_eq o1 o2)) <==> (va_eval_opr64 s o1 == va_eval_opr64 s o2))
   [SMTPat (eval_ocmp s (va_cmp_eq o1 o2))]
 
-val lemma_cmp_ne : s:va_state -> o1:va_operand{ not (TMem? o1 || TStack? o1) } -> o2:va_operand{ not (TMem? o2 || TStack? o2) } -> Lemma
+val lemma_cmp_ne : s:va_state -> o1:va_operand{ not (OMem? o1 || OStack? o1) } -> o2:va_operand{ not (OMem? o2 || OStack? o2) } -> Lemma
   (requires True)
   (ensures  (eval_ocmp s (va_cmp_ne o1 o2)) <==> (va_eval_opr64 s o1 <> va_eval_opr64 s o2))
   [SMTPat (eval_ocmp s (va_cmp_ne o1 o2))]
 
-val lemma_cmp_le : s:va_state -> o1:va_operand{ not (TMem? o1 || TStack? o1) } -> o2:va_operand{ not (TMem? o2 || TStack? o2) } -> Lemma
+val lemma_cmp_le : s:va_state -> o1:va_operand{ not (OMem? o1 || OStack? o1) } -> o2:va_operand{ not (OMem? o2 || OStack? o2) } -> Lemma
   (requires True)
   (ensures  (eval_ocmp s (va_cmp_le o1 o2)) <==> (va_eval_opr64 s o1 <= va_eval_opr64 s o2))
   [SMTPat (eval_ocmp s (va_cmp_le o1 o2))]
 
-val lemma_cmp_ge : s:va_state -> o1:va_operand{ not (TMem? o1 || TStack? o1) } -> o2:va_operand{ not (TMem? o2 || TStack? o2) } -> Lemma
+val lemma_cmp_ge : s:va_state -> o1:va_operand{ not (OMem? o1 || OStack? o1) } -> o2:va_operand{ not (OMem? o2 || OStack? o2) } -> Lemma
   (requires True)
   (ensures  (eval_ocmp s (va_cmp_ge o1 o2)) <==> (va_eval_opr64 s o1 >= va_eval_opr64 s o2))
   [SMTPat (eval_ocmp s (va_cmp_ge o1 o2))]
 
-val lemma_cmp_lt : s:va_state -> o1:va_operand{ not (TMem? o1 || TStack? o1) } -> o2:va_operand{ not (TMem? o2 || TStack? o2) } -> Lemma
+val lemma_cmp_lt : s:va_state -> o1:va_operand{ not (OMem? o1 || OStack? o1) } -> o2:va_operand{ not (OMem? o2 || OStack? o2) } -> Lemma
   (requires True)
   (ensures  (eval_ocmp s (va_cmp_lt o1 o2)) <==> (va_eval_opr64 s o1 < va_eval_opr64 s o2))
   [SMTPat (eval_ocmp s (va_cmp_lt o1 o2))]
 
-val lemma_cmp_gt : s:va_state -> o1:va_operand{ not (TMem? o1 || TStack? o1) } -> o2:va_operand{ not (TMem? o2 || TStack? o2) } -> Lemma
+val lemma_cmp_gt : s:va_state -> o1:va_operand{ not (OMem? o1 || OStack? o1) } -> o2:va_operand{ not (OMem? o2 || OStack? o2) } -> Lemma
   (requires True)
   (ensures  (eval_ocmp s (va_cmp_gt o1 o2)) <==> (va_eval_opr64 s o1 > va_eval_opr64 s o2))
   [SMTPat (eval_ocmp s (va_cmp_gt o1 o2))]
 
-val lemma_valid_cmp_eq : s:va_state -> o1:va_operand{ not (TMem? o1 || TStack? o1) } -> o2:va_operand{ not (TMem? o2 || TStack? o2) } -> Lemma
+val lemma_valid_cmp_eq : s:va_state -> o1:va_operand{ not (OMem? o1 || OStack? o1) } -> o2:va_operand{ not (OMem? o2 || OStack? o2) } -> Lemma
   (requires True)
   (ensures  (valid_operand o1 s /\ valid_operand o2 s) ==> (valid_ocmp (va_cmp_eq o1 o2) s))
   [SMTPat (valid_ocmp (va_cmp_eq o1 o2) s)]
 
-val lemma_valid_cmp_ne : s:va_state -> o1:va_operand{ not (TMem? o1 || TStack? o1) } -> o2:va_operand{ not (TMem? o2 || TStack? o2) } -> Lemma
+val lemma_valid_cmp_ne : s:va_state -> o1:va_operand{ not (OMem? o1 || OStack? o1) } -> o2:va_operand{ not (OMem? o2 || OStack? o2) } -> Lemma
   (requires True)
   (ensures (valid_operand o1 s /\ valid_operand o2 s) ==> (valid_ocmp (va_cmp_ne o1 o2) s))
   [SMTPat (valid_ocmp (va_cmp_ne o1 o2) s)]
 
-val lemma_valid_cmp_le : s:va_state -> o1:va_operand{ not (TMem? o1 || TStack? o1) } -> o2:va_operand{ not (TMem? o2 || TStack? o2) } -> Lemma
+val lemma_valid_cmp_le : s:va_state -> o1:va_operand{ not (OMem? o1 || OStack? o1) } -> o2:va_operand{ not (OMem? o2 || OStack? o2) } -> Lemma
   (requires True)
   (ensures (valid_operand o1 s /\ valid_operand o2 s) ==> (valid_ocmp (va_cmp_le o1 o2) s))
   [SMTPat (valid_ocmp (va_cmp_le o1 o2) s)]
 
-val lemma_valid_cmp_ge : s:va_state -> o1:va_operand{ not (TMem? o1 || TStack? o1) } -> o2:va_operand{ not (TMem? o2 || TStack? o2) } -> Lemma
+val lemma_valid_cmp_ge : s:va_state -> o1:va_operand{ not (OMem? o1 || OStack? o1) } -> o2:va_operand{ not (OMem? o2 || OStack? o2) } -> Lemma
   (requires True)
   (ensures (valid_operand o1 s /\ valid_operand o2 s) ==> (valid_ocmp (va_cmp_ge o1 o2) s))
   [SMTPat (valid_ocmp (va_cmp_ge o1 o2) s)]
 
-val lemma_valid_cmp_lt : s:va_state -> o1:va_operand{ not (TMem? o1 || TStack? o1) } -> o2:va_operand{ not (TMem? o2 || TStack? o2) } -> Lemma
+val lemma_valid_cmp_lt : s:va_state -> o1:va_operand{ not (OMem? o1 || OStack? o1) } -> o2:va_operand{ not (OMem? o2 || OStack? o2) } -> Lemma
   (requires True)
   (ensures (valid_operand o1 s /\ valid_operand o2 s) ==> (valid_ocmp (va_cmp_lt o1 o2) s))
   [SMTPat (valid_ocmp (va_cmp_lt o1 o2) s)]
 
-val lemma_valid_cmp_gt : s:va_state -> o1:va_operand{ not (TMem? o1 || TStack? o1) } -> o2:va_operand{ not (TMem? o2 || TStack? o2) } -> Lemma
+val lemma_valid_cmp_gt : s:va_state -> o1:va_operand{ not (OMem? o1 || OStack? o1) } -> o2:va_operand{ not (OMem? o2 || OStack? o2) } -> Lemma
   (requires True)
   (ensures (valid_operand o1 s /\ valid_operand o2 s) ==> (valid_ocmp (va_cmp_gt o1 o2) s))
   [SMTPat (valid_ocmp (va_cmp_gt o1 o2) s)]
@@ -709,10 +658,9 @@ val gcc : printer
 
 unfold let memTaint_type = Map.t int taint
 
-// There can only be one!
 [@va_qattr]
 let max_one_mem (o1 o2:va_operand) : prop0 =
   match (o1, o2) with
-  | (TMem _ _, TMem _ _) | (TMem _ _, TStack _ _) | (TStack _ _, TMem _ _) | (TStack _ _, TStack _ _) -> False
+  | (OMem _, OMem _) | (OMem _, OStack _) | (OStack _, OMem _) | (OStack _, OStack _) -> False
   | _ -> True
 
