vale/code/arch/x64/X64.Leakage_Helpers.fst
@@ -10,35 +10,35 @@ let merge_taint (t1:taint) (t2:taint) :taint =
   else Public
 
 (* Also pass the taint of the instruction *)
-let operand_taint (op:operand) ts taint =
+let operand_taint (op:operand) (ts:analysis_taints) =
   match op with
-    | OConst _ -> Public
-    | OReg reg -> ts.regTaint reg
-    | OMem _ | OStack _ -> taint
+  | OConst _ -> Public
+  | OReg reg -> ts.regTaint reg
+  | OMem (_, t) | OStack (_, t) -> t
 
-let operand_taint128 (op:mov128_op) (ts:analysis_taints) (t:taint) : taint =
+let operand_taint128 (op:operand128) (ts:analysis_taints) : taint =
   match op with
-  | Mov128Xmm x -> ts.xmmTaint x
-  | Mov128Mem _ | Mov128Stack _ -> t
+  | OReg128 x -> ts.xmmTaint x
+  | OMem128 (_, t) | OStack128 (_, t) -> t
 
 [@instr_attr]
 let operand_taint_explicit
   (i:instr_operand_explicit)
   (o:instr_operand_t i)
   (ts:analysis_taints)
-  (t:taint) : taint =
+  : taint =
   match i with
-  | IOp64 -> operand_taint o ts t
-  | IOpXmm -> operand_taint128 o ts t
+  | IOp64 -> operand_taint o ts
+  | IOpXmm -> operand_taint128 o ts
 
 [@instr_attr]
 let operand_taint_implicit
   (i:instr_operand_implicit)
   (ts:analysis_taints)
-  (t:taint) : taint =
+  : taint =
   match i with
-  | IOp64One o -> operand_taint o ts t
-  | IOpXmmOne o -> operand_taint128 o ts t
+  | IOp64One o -> operand_taint o ts
+  | IOpXmmOne o -> operand_taint128 o ts
   | IOpFlagsCf -> ts.cfFlagsTaint
   | IOpFlagsOf -> ts.ofFlagsTaint
 
@@ -47,17 +47,19 @@ let rec args_taint
   (args:list instr_operand)
   (oprs:instr_operands_t_args args)
   (ts:analysis_taints)
-  (t:taint) : taint =
+  : taint =
   match args with
   | [] -> Public
   | i::args ->
     match i with
-    | IOpEx i -> let oprs = coerce oprs in merge_taint
-                (operand_taint_explicit i (fst oprs) ts t)
-                (args_taint args (snd oprs) ts t)
-    | IOpIm i -> merge_taint
-            (operand_taint_implicit i ts t)
-            (args_taint args (coerce oprs) ts t)
+    | IOpEx i ->
+      let oprs = coerce oprs in merge_taint
+      (operand_taint_explicit i (fst oprs) ts)
+      (args_taint args (snd oprs) ts)
+    | IOpIm i ->
+      merge_taint
+      (operand_taint_implicit i ts)
+      (args_taint args (coerce oprs) ts)
 
 [@instr_attr]
 let rec inouts_taint
@@ -65,72 +67,65 @@ let rec inouts_taint
   (args:list instr_operand)
   (oprs:instr_operands_t inouts args)
   (ts:analysis_taints)
-  (t:taint) : taint =
+  : taint =
   match inouts with
-  | [] -> args_taint args oprs ts t
+  | [] -> args_taint args oprs ts
   | (Out, i)::inouts ->
     let oprs =
       match i with
       | IOpEx i -> snd #(instr_operand_t i) (coerce oprs)
       | IOpIm i -> coerce oprs
-    in inouts_taint inouts args oprs ts t
+    in inouts_taint inouts args oprs ts
   | (InOut, i)::inouts -> 
     let (v, oprs) =
       match i with
-      | IOpEx i -> let oprs = coerce oprs in
-              (operand_taint_explicit i (fst oprs) ts t), snd oprs
-      | IOpIm i -> operand_taint_implicit i ts t, coerce oprs
-    in merge_taint v (inouts_taint inouts args oprs ts t)
+      | IOpEx i ->
+        let oprs = coerce oprs in
+        ((operand_taint_explicit i (fst oprs) ts), snd oprs)
+      | IOpIm i -> (operand_taint_implicit i ts, coerce oprs)
+    in merge_taint v (inouts_taint inouts args oprs ts)
 
-
-let maddr_does_not_use_secrets addr ts =
+let maddr_does_not_use_secrets (addr:maddr) (ts:analysis_taints) : bool =
   match addr with
-    | MConst _ -> true
-    | MReg r _ -> Public? (operand_taint (OReg r) ts Public)
-    | MIndex base _ index _ ->
-        let baseTaint = operand_taint (OReg base) ts Public in
-        let indexTaint = operand_taint (OReg index) ts Public in
-        (Public? baseTaint) && (Public? indexTaint)
+  | MConst _ -> true
+  | MReg r _ -> Public? (operand_taint (OReg r) ts)
+  | MIndex base _ index _ ->
+      let baseTaint = operand_taint (OReg base) ts in
+      let indexTaint = operand_taint (OReg index) ts in
+      (Public? baseTaint) && (Public? indexTaint)
 
-let operand_does_not_use_secrets op ts =
+let operand_does_not_use_secrets (op:operand) (ts:analysis_taints) : bool =
   match op with
   | OConst _ | OReg _ -> true 
-  | OMem m | OStack m -> maddr_does_not_use_secrets m ts
+  | OMem (m, _) | OStack (m, _) -> maddr_does_not_use_secrets m ts
 
-let operand128_does_not_use_secrets (op:mov128_op) (ts:analysis_taints) : bool =
+let operand128_does_not_use_secrets (op:operand128) (ts:analysis_taints) : bool =
   match op with
-  | Mov128Xmm _ -> true
-  | Mov128Mem m | Mov128Stack m -> maddr_does_not_use_secrets m ts
+  | OReg128 _ -> true
+  | OMem128 (m, _) | OStack128 (m, _) -> maddr_does_not_use_secrets m ts
 
-let operand_taint_allowed (o:operand) (t_operand t_data:taint) : bool =
+let operand_taint_allowed (o:operand) (t_data:taint) : bool =
   match o with
   | OConst _ | OReg _ -> true
-  | OMem _ | OStack _ -> t_operand = Secret || t_data = Public
+  | OMem (_, t_operand) | OStack (_, t_operand) -> t_operand = Secret || t_data = Public
 
-let operand128_taint_allowed (o:mov128_op) (t_operand t_data:taint) : bool =
+let operand128_taint_allowed (o:operand128) (t_data:taint) : bool =
   match o with
-  | Mov128Xmm _ -> true
-  | Mov128Mem _ | Mov128Stack _ -> t_operand = Secret || t_data = Public
+  | OReg128 _ -> true
+  | OMem128 (_, t_operand) | OStack128 (_, t_operand) -> t_operand = Secret || t_data = Public
 
-val lemma_operand_obs:  (ts:analysis_taints) ->  (dst:operand) -> (s1 : machine_state) -> (s2:machine_state) -> Lemma ((operand_does_not_use_secrets dst ts) /\ publicValuesAreSame ts s1 s2 ==> (operand_obs s1 dst) = (operand_obs s2 dst))
-
-#reset-options "--initial_ifuel 2 --max_ifuel 2 --initial_fuel 4 --max_fuel 4 --z3rlimit 20"
-let lemma_operand_obs ts dst s1 s2 = match dst with
-  | OConst _ | OReg _ -> ()
-  | OMem m | OStack m  -> ()
-#reset-options "--initial_ifuel 2 --max_ifuel 2 --initial_fuel 4 --max_fuel 4 --z3rlimit 5"
-
-let set_taint (dst:operand) ts taint : Tot analysis_taints =
+let set_taint (dst:operand) (ts:analysis_taints) (t:taint) : analysis_taints =
   match dst with
-  | OConst _ -> ts  (* Shouldn't actually happen *)
-  | OReg r -> AnalysisTaints (FunctionalExtensionality.on reg (fun x -> if x = r then taint else ts.regTaint x)) ts.flagsTaint ts.cfFlagsTaint ts.ofFlagsTaint ts.xmmTaint
-  | OMem m | OStack m -> ts (* Ensured by taint semantics *)
+  | OConst _ -> ts  // Shouldn't actually happen
+  | OReg r -> AnalysisTaints (FunctionalExtensionality.on reg
+      (fun x -> if x = r then t else ts.regTaint x)) ts.flagsTaint ts.cfFlagsTaint ts.ofFlagsTaint ts.xmmTaint
+  | OMem _ | OStack _ -> ts (* Ensured by taint semantics *)
 
-let set_taint128 (dst:mov128_op) (ts:analysis_taints) (t:taint) : analysis_taints =
+let set_taint128 (dst:operand128) (ts:analysis_taints) (t:taint) : analysis_taints =
   match dst with
-  | Mov128Xmm r -> AnalysisTaints ts.regTaint ts.flagsTaint ts.cfFlagsTaint ts.ofFlagsTaint
+  | OReg128 r -> AnalysisTaints ts.regTaint ts.flagsTaint ts.cfFlagsTaint ts.ofFlagsTaint
       (FunctionalExtensionality.on xmm (fun x -> if x = r then t else ts.xmmTaint x))
-  | Mov128Mem _ | Mov128Stack _-> ts
+  | OMem128 _ | OStack128 _-> ts
 
 let set_taint_cf_and_flags (ts:analysis_taints) (t:taint) : analysis_taints =
   let AnalysisTaints rs flags cf ovf xmms = ts in
@@ -144,61 +139,11 @@ let rec operands_do_not_use_secrets ops ts = match ops with
   | [] -> true
   | hd :: tl -> operand_does_not_use_secrets hd ts && (operands_do_not_use_secrets tl ts)
 
-val lemma_operands_imply_op: (ts:analysis_taints) -> (ops:list operand{Cons? ops}) -> Lemma
-  (requires (operands_do_not_use_secrets ops ts))
-  (ensures (operand_does_not_use_secrets (List.Tot.Base.hd ops) ts))
-
-let lemma_operands_imply_op ts ops = match ops with
-  | hd :: tl -> ()
-
-let ins_consumes_fixed_time (ins : tainted_ins) (ts:analysis_taints) (res:bool*analysis_taints) =
+let ins_consumes_fixed_time (ins : ins) (ts:analysis_taints) (res:bool*analysis_taints) =
   let b, ts' = res in
   ((b2t b) ==> isConstantTime (Ins ins) ts)
 
-
-(*val lemma_operand_obs_list: (ts:analysis_taints) -> (ops:list operand) -> (s1:machine_state) -> (s2:machine_state) -> Lemma  ((operands_do_not_use_secrets ops ts /\ publicValuesAreSame ts s1 s2) ==>
-  (operand_obs_list s1 ops) == (operand_obs_list s2 ops))
-
-let rec lemma_operand_obs_list ts ops s1 s2 = match ops with
-  | [] -> ()
-  | hd :: tl -> lemma_operand_obs_list ts tl s1 s2
-
-
-let rec sources_taint srcs ts taint = match srcs with
-  | [] -> taint
-  | hd :: tl -> merge_taint (operand_taint hd ts taint) (sources_taint tl ts taint)
-
-let rec set_taints dsts ts taint = match dsts with
-  | [] -> ts
-  | hd :: tl -> set_taints tl (set_taint hd ts taint) taint
-
-val lemma_taint_sources: (ins:tainted_ins) -> (ts:analysis_taints) -> Lemma
-(let i = ins.i in
- let d, s = extract_operands i in
-forall src. List.Tot.Base.mem src s /\ Public? (sources_taint s ts ins.t) ==> Public? (operand_taint src ts ins.t))
-
-let lemma_taint_sources ins ts = ()
-*)
 #set-options "--z3rlimit 20"
-
-val lemma_public_op_are_same:
-  (ts:analysis_taints) -> (op:operand) -> (s1:machine_state) -> (s2:machine_state)
-   -> Lemma (requires (operand_does_not_use_secrets op ts   /\
-                      Public? (operand_taint op ts Public) /\
-		      publicValuesAreSame ts s1 s2         /\
-		      taint_match op Public s1.ms_memTaint s1.ms_stackTaint s1 /\
-		      taint_match op Public s2.ms_memTaint s2.ms_stackTaint s2))
-           (ensures eval_operand op s1 == eval_operand op s2)
-let lemma_public_op_are_same ts op s1 s2 =
-  match op with
-  | OConst _ -> ()
-  | OReg _ -> ()
-  | OMem m | OStack m ->
-    let a1 = eval_maddr m s1 in
-    let a2 = eval_maddr m s2 in
-    assert (a1 == a2);
-//    assert (forall a. (a >= a1 /\ a < a1 + 8) ==> s1.ms_mem.[a] == s2.ms_mem.[a]);
-    Opaque_s.reveal_opaque get_heap_val64_def
 
 val publicFlagValuesAreAsExpected: (tsAnalysis:analysis_taints) -> (tsExpected:analysis_taints) -> b:bool{b <==> (Public? tsExpected.flagsTaint ==> Public? tsAnalysis.flagsTaint)}
 
