vale/code/arch/x64/X64.Taint_Semantics.fst
@@ -10,47 +10,14 @@ module L = FStar.List.Tot
 let normal_term_spec (#a:Type) (x:a) : Lemma (normal x == x) =
   ()
 
-let mk_ins (i:S.ins) (t:taint) : Pure tainted_code
+let mk_ins (i:S.ins) : Pure tainted_code
   (requires True)
   (ensures fun c ->
-    c == Ins (TaintedIns i t) /\
+    c == Ins i /\
     i == normal i /\
     S.eval_ins i == normal (S.eval_ins i)
   )
   =
   normal_term_spec (S.eval_ins i);
-  Ins (TaintedIns i t)
+  Ins i
 
-let mk_taint_ins1 (i:operand->S.ins)
-                  (o:va_operand)
-                  : tainted_code
-  =
-  let o_basic = t_op_to_op o in
-  Ins (TaintedIns (i o_basic) (get_taint o))
-
-let mk_taint_ins2 (i:operand->operand->S.ins)
-                  (o1 o2:va_operand)
-                  : tainted_code
-  =
-  let o1_basic = t_op_to_op o1 in
-  let o2_basic = t_op_to_op o2 in
-  Ins (TaintedIns (i o1_basic o2_basic)
-                  (extract_taint o1 o2))
-
-let mk_taint_ins3 (i:operand->operand->operand->S.ins)
-                  (o1 o2 o3:va_operand)
-                  : tainted_code
-  =
-  let o1_basic = t_op_to_op o1 in
-  let o2_basic = t_op_to_op o2 in
-  let o3_basic = t_op_to_op o3 in
-  Ins (TaintedIns (i o1_basic o2_basic o3_basic)
-                  (extract_taint3 o1 o2 o3))
-
-let mk_taint128_ins2 (i:mov128_op->mov128_op->S.ins)
-                     (o1 o2:va_operand128)
-                    : tainted_code
-  =
-  let o1_basic = t_op_to_op128 o1 in
-  let o2_basic = t_op_to_op128 o2 in
-  Ins (TaintedIns (i o1_basic o2_basic) (extract_taint128 o1 o2))
