vale/code/arch/x64/X64.Vale.InsLemmas.fsti
@@ -3,14 +3,31 @@ module X64.Vale.InsLemmas
 open X64.Machine_s
 open X64.Instruction_s
 open X64.Vale.State
+open X64.Vale.StateLemmas
 open X64.Vale.Decls
 module BC = X64.Bytes_Code_s
 module S = X64.Bytes_Semantics_s
+module TS = X64.Taint_Semantics_s
+
+let has_taint128 (o:operand128) (t:taint) : bool =
+  match o with
+  | OMem128 (_, t') | OStack128 (_, t') -> t = t'
+  | _ -> true
 
 val lemma_valid_taint64_operand (m:maddr) (t:taint) (s:va_state) : Lemma
-  (requires valid_operand (TMem m t) s)
+  (requires valid_operand (OMem (m, t)) s)
   (ensures taint_at s.memTaint (eval_maddr m s) == t)
-  [SMTPat (eval_maddr m s); SMTPat (TMem m t)]
+  [SMTPat (eval_maddr m s); SMTPat (OMem (m, t))]
+
+val lemma_valid_taint_match64 (o:operand) (s:state) : Lemma
+  (requires valid_operand o s)
+  (ensures TS.taint_match o s.memTaint s.stackTaint (state_to_S s))
+  [SMTPat (TS.taint_match o s.memTaint s.stackTaint (state_to_S s))]
+
+val lemma_valid_taint_match128 (o:operand128) (s:state) : Lemma
+  (requires valid_operand128 o s)
+  (ensures TS.taint_match128 o s.memTaint s.stackTaint (state_to_S s))
+  [SMTPat (TS.taint_match128 o s.memTaint s.stackTaint (state_to_S s))]
 
 [@instr_attr]
 let rec make_instr_t_args (args:list instr_operand) : Type0 =
